examples/crypto/cryptobox/Box.Indexing.fst
@@ -1,31 +1,83 @@
 module Box.Indexing
 
 open FStar.Set
+open FStar.Heap
 open FStar.HyperHeap
+open FStar.HyperStack
+
+module MR = FStar.Monotonic.RRef
+module MM = MonotoneMap
+
 
 // Make these abstract!
 type id = UInt32.t
-type ae_id = (id*id)
+private type range = fun id -> bool
+private let inv (f:MM.map' id range) = True
+private let table = MM.alloc #root #id #range #inv 
 
-//type log_t: (r:rid) = 
-//  Log: m_rref r (seq id) grows
-//
-//val log: log_t
+
+//abstract type val honest: i:id -> Tot bool
+let honest (i:id) =
+  MR.witnessed (MM.contains table i true)
+
+let dishonest (i:id) =
+  MR.witnessed (MM.contains table i false)
+
+assume val lemma_dis_implies_not: i:id -> Lemma 
+  (requires (True))
+  (ensures (dishonest i ==> ~(honest i)))
+  [SMTPat (dishonest i) ]
+
+
+val honestST: i:id -> St(b:bool{(b ==> honest i) /\ (not b ==> dishonest i)})
+let honestST (i:id) =
+  MR.m_recall table;
+  match MM.lookup table i with
+  |Some v -> 
+    v=true
+  |None -> 
+    MM.extend table i false;
+    false
+
+type ae_id = (id*id)
+private type ae_range = fun (i:ae_id) -> (b:bool{b ==> honest (fst i) /\ honest (snd i)})
+private let ae_inv (f:MM.map' ae_id ae_range) = True
+private let ae_table = MM.alloc #root #ae_id #ae_range #ae_inv 
+
+
 
 assume val generate_ae_id: i1:id -> i2:id -> Tot (i3:ae_id{i3=(i1,i2)})
 
-assume val honest: i:id -> Tot bool
-//let honest i =
-//  let root = HyperHeap.get() in
-//  if m_contains log root then
-//    let id_log = m_read log in
-//    match seq_find (fun entry -> entry = i) id_log with
-//    | Some i' -> true
-//    | None -> false
-//  else
-//    log =
 
-assume val ae_honest: i:ae_id -> Tot (b:bool{b ==> (honest (fst i) /\ honest (snd i))})
+//assume val ae_honest: i:ae_id -> Tot (b:bool{b ==> (honest (fst i) /\ honest (snd i))})
+let ae_honest (i:ae_id) =
+  honest (fst i) /\ honest (snd i) /\
+  MR.witnessed (MM.contains ae_table i true)
+
+let ae_dishonest (i:ae_id) =
+  dishonest (fst i) \/ dishonest (snd i) \/
+  MR.witnessed (MM.contains ae_table i false)
+
+assume val lemma_ae_dis_implies_not: i:ae_id -> Lemma 
+  (requires (True))
+  (ensures (ae_dishonest i ==> ~(ae_honest i)))
+  [SMTPat (ae_dishonest i) ]
+  
+val ae_honestST: i:ae_id -> ST(b:bool{(b ==> ae_honest i) /\ (not b ==> ae_dishonest i)})
+  (requires (fun h0 -> True))
+  (ensures (fun h0 t h1 -> 
+    modifies (Set.singleton root) h0 h1 // precise enough?
+    ))
+let ae_honestST (i:ae_id) =
+  MR.m_recall ae_table;
+  match MM.lookup ae_table i with
+  |Some v -> 
+    v=true
+  |None -> 
+    MM.extend ae_table i false;
+    false
+
+
 //val ae_honest: i:ae_id -> Tot (b:bool ==> (forall x. mem x i ==> honest x))
 
 assume Index_hasEq: hasEq id
